Update ADT.v

ADT.v
@@ -1,4 +1,4 @@
-From Coq Require Import String.  
+From Coq Require Import String.   
 From VFA Require Import Perm.
 From VFA Require Import Maps.
 From VFA Require Import SearchTree.
@@ -195,6 +195,685 @@ Proof.
 Qed.
 
 End TreeTable.
+
+Module Type ETable_first_attempt.
+
+Include Table.
+
+Parameter bound : key -> table -> bool.
+Parameter elements : table -> list (key * V).
+
+Axiom elements_complete : forall (k : key) (v : V) (t : table),
+  bound k t = true ->
+  get k t = v ->
+  In (k, v) (elements t).
+
+Axiom elements_correct : forall (k : key) (v : V) (t : table),
+  In (k, v) (elements t) ->
+  bound k t = true /\ get k t = v.
+
+End ETable_first_attempt.
+
+Module TreeETable_first_attempt (VT : ValType) <: ETable_first_attempt.
+
+Include TreeTable VT.
+
+Check get : key -> table -> V.
+
+Definition bound (k : key) (t : table) : bool :=
+    SearchTree.bound k t.
+
+Definition elements (t : table) : list (key * V) :=
+    SearchTree.elements t.
+
+Theorem elements_complete : forall (k : key) (v : V) (t : table),
+      bound k t = true ->
+      get k t = v ->
+      In (k, v) (elements t).
+Proof.
+intros k v t Hbound Hlookup. unfold get in Hlookup.
+pose proof (SearchTree.elements_complete) as Hcomplete.
+unfold elements_complete_spec in Hcomplete. 
+apply Hcomplete with default. 
+(* Stuck *)
+Admitted.
+
+Theorem elements_correct : forall (k : key) (v : V) (t : table),
+   In (k, v) (elements t) ->
+   bound k t = true /\ get k t = v.
+Proof.
+intros k v t Hin.
+pose proof (SearchTree.elements_correct) as Hcorrect.
+unfold elements_correct_spec in Hcorrect.
+apply Hcorrect.
+Admitted.
+
+End TreeETable_first_attempt.
+
+Module Type ETable.
+Include Table.
+  
+Parameter rep_ok : table -> Prop.
+Parameter bound : key -> table -> bool.
+Parameter elements : table -> list (key * V).
+
+Axiom empty_ok : rep_ok empty.
+
+Axiom set_ok : forall (k : key) (v : V) (t : table),
+      rep_ok t -> rep_ok (set k v t).
+
+Axiom bound_empty : forall (k : key),
+      bound k empty = false.
+
+Axiom bound_set_same : forall (k : key) (v : V) (t : table),
+      bound k (set k v t) = true.
+
+Axiom bound_set_other : forall (k k' : key) (v : V) (t : table),
+      k <> k' -> bound k' (set k v t) = bound k' t.
+
+Axiom elements_complete : forall (k : key) (v : V) (t : table),
+      rep_ok t ->
+      bound k t = true ->
+      get k t = v ->
+      In (k, v) (elements t).
+
+Axiom elements_correct : forall (k : key) (v : V) (t : table),
+      rep_ok t ->
+      In (k, v) (elements t) ->
+      bound k t = true /\ get k t = v.
+
+End ETable.
+
+Module TreeETable (VT : ValType) <: ETable.
+Include TreeTable VT.
+
+Definition rep_ok (t : table) : Prop :=
+    BST t.
+
+Definition bound (k : key) (t : table) : bool :=
+    SearchTree.bound k t.
+
+Definition elements (t : table) : list (key * V) :=
+    SearchTree.elements t.
+
+Theorem empty_ok : rep_ok empty.
+Proof. 
+unfold rep_ok. unfold empty. unfold empty_tree. apply BST_E.
+Qed. 
+
+Theorem set_ok : forall (k : key) (v : V) (t : table),
+      rep_ok t -> rep_ok (set k v t).
+Proof.
+apply insert_BST.
+Qed.
+
+Theorem bound_empty : forall (k : key),
+      bound k empty = false.
+Proof.
+reflexivity.
+Qed.
+
+Theorem bound_set_same : forall (k : key) (v : V) (t : table),
+      bound k (set k v t) = true.
+Proof.
+intros k v t. unfold bound, set. induction t; bdall.
+Qed.
+
+Theorem bound_set_other : forall (k k' : key) (v : V) (t : table),
+      k <> k' -> bound k' (set k v t) = bound k' t.
+Proof.
+intros k k' v t Hneq. unfold bound, set. induction t; bdall.
+Qed.
+
+Theorem elements_complete : forall (k : key) (v : V) (t : table),
+      rep_ok t ->
+      bound k t = true ->
+      get k t = v ->
+      In (k, v) (elements t).
+Proof.
+intros k v t Hbound Hlookup.
+pose proof SearchTree.elements_complete as Hcomplete.
+unfold elements_complete_spec in Hcomplete. unfold get.  
+apply Hcomplete. apply Hlookup.
+Qed.
+
+Theorem elements_correct : forall (k : key) (v : V) (t : table),
+      rep_ok t ->
+      In (k, v) (elements t) ->
+      bound k t = true /\ get k t = v.
+Proof.
+intros k v t. simpl. intros Hin.
+pose proof SearchTree.elements_correct as Hcorrect.
+unfold elements_correct_spec in Hcorrect.
+apply Hcorrect; assumption.
+Qed.
+
+End TreeETable.
+
+Module StringTreeETableExample.
+
+Module StringTreeETable := TreeETable StringVal.
+Import StringTreeETable.
+Open Scope string_scope.
+
+Example ex1 :
+   In (0, "A") (elements (set 0 "A" (set 1 "B" empty))).
+Proof.
+apply elements_complete;
+auto using empty_ok, set_ok, bound_set_same, get_set_same.
+Qed.
+
+End StringTreeETableExample.
+
+Module TreeETableFullyEncapsulated (VT : ValType) : ETable.
+Include TreeTable VT.
+
+Definition rep_ok (t : table) : Prop :=
+    BST t.
+
+Definition bound (k : key) (t : table) : bool :=
+    SearchTree.bound k t.
+
+Definition elements (t : table) : list (key * V) :=
+    SearchTree.elements t.
+
+Theorem empty_ok : rep_ok empty.
+Proof.
+apply empty_tree_BST.
+Qed.
+
+Theorem set_ok : forall (k : key) (v : V) (t : table),
+   rep_ok t -> rep_ok (set k v t).
+Proof.
+apply insert_BST.
+Qed.
+
+Theorem bound_empty : forall (k : key),
+   bound k empty = false.
+Proof.
+reflexivity.
+Qed.
+
+Theorem bound_set_same : forall (k : key) (v : V) (t : table),
+  bound k (set k v t) = true.
+Proof.
+  intros k v t. unfold bound, set. induction t; bdall.
+Qed.
+
+Theorem bound_set_other : forall (k k' : key) (v : V) (t : table),
+  k <> k' -> bound k' (set k v t) = bound k' t.
+Proof.
+  intros k k' v t Hneq. unfold bound, set. induction t; bdall.
+Qed.
+
+Theorem elements_complete : forall (k : key) (v : V) (t : table),
+   rep_ok t ->
+   bound k t = true ->
+   get k t = v ->
+   In (k, v) (elements t).
+Proof.
+  intros k v t Hbound Hlookup.
+  pose proof SearchTree.elements_complete as Hcomplete.
+  unfold elements_complete_spec in Hcomplete.
+  apply Hcomplete; assumption.
+Qed.
+
+Theorem elements_correct : forall (k : key) (v : V) (t : table),
+  rep_ok t ->
+  In (k, v) (elements t) ->
+  bound k t = true /\ get k t = v.
+Proof.
+  intros k v t. simpl. intros Hin.
+  pose proof SearchTree.elements_correct as Hcorrect.
+  unfold elements_correct_spec in Hcorrect.
+  apply Hcorrect; assumption.
+Qed.
+
+End TreeETableFullyEncapsulated.
+
+Module OverlyEncapsulatedExample.
+
+Module StringTreeETableFullyEncapsulated := TreeETableFullyEncapsulated StringVal.
+Import StringTreeETableFullyEncapsulated.
+Open Scope string_scope.
+
+Fail Example ex1 : get 0 empty = "".
+  (* fails with an error about "" not having type V *)
+End OverlyEncapsulatedExample.
+
+Print OverlyEncapsulatedExample.StringTreeETableFullyEncapsulated.V.
+
+Module Type SimpleTable.
+  Parameter key : Type.
+  Parameter V : Type.
+  Parameter default : V.
+  Parameter table : Type.
+End SimpleTable.
+
+Module SimpleStringTable1 : SimpleTable.
+  Definition key := nat.
+  Definition V := string.
+  Definition default : string := "".
+  Definition table := tree V.
+End SimpleStringTable1.
+(* V is abstract. *)
+Print SimpleStringTable1.V.
+
+Module Type SimpleTable2 := SimpleTable with Definition V := string.
+
+Module SimpleStringTable2 : SimpleTable2.
+  Definition key := nat.
+  Definition V := string.
+  Definition default : string := "".
+  Definition table := tree V.
+End SimpleStringTable2.
+
+(* V is exposed, but default is abstract. *)
+Print SimpleStringTable2.V.
+Print SimpleStringTable2.default.
+
+Module Type SimpleTable3 := SimpleTable
+  with Definition V := string
+  with Definition default := ""%string.
+
+Module SimpleStringTable3 : SimpleTable3.
+  Definition key := nat.
+  Definition V := string.
+  Definition default : string := "".
+  Definition table := tree V.
+End SimpleStringTable3.
+
+(* Both V and default are exposed. *)
+Print SimpleStringTable3.V.
+Print SimpleStringTable3.default.
+
+Module TreeETableEncapsulated (VT : ValType) : (ETable with Definition V := VT.V with Definition default := VT.default).
+Include TreeTable VT.
+
+Definition rep_ok (t : table) : Prop :=
+    BST t.
+  
+Definition bound (k : key) (t : table) : bool :=
+    SearchTree.bound k t.
+
+Definition elements (t : table) : list (key * V) :=
+    SearchTree.elements t.
+
+Theorem empty_ok : rep_ok empty.
+Proof.
+  apply empty_tree_BST.
+Qed.
+
+Theorem set_ok : forall (k : key) (v : V) (t : table),
+   rep_ok t -> rep_ok (set k v t).
+Proof.
+  apply insert_BST.
+Qed.
+
+Theorem bound_empty : forall (k : key),
+  bound k empty = false.
+Proof.
+  reflexivity.
+Qed.
+
+Theorem bound_set_same : forall (k : key) (v : V) (t : table),
+  bound k (set k v t) = true.
+Proof.
+  intros k v t. unfold bound, set. induction t; bdall.
+Qed.
+
+Theorem bound_set_other : forall (k k' : key) (v : V) (t : table),
+      k <> k' -> bound k' (set k v t) = bound k' t.
+Proof.
+  intros k k' v t Hneq. unfold bound, set. induction t; bdall.
+Qed.
+
+Theorem elements_complete : forall (k : key) (v : V) (t : table),
+    rep_ok t ->
+    bound k t = true ->
+    get k t = v ->
+    In (k, v) (elements t).
+Proof.
+  intros k v t Hbound Hlookup.
+  pose proof SearchTree.elements_complete as Hcomplete.
+  unfold elements_complete_spec in Hcomplete.
+  apply Hcomplete; assumption.
+Qed.
+
+Theorem elements_correct : forall (k : key) (v : V) (t : table),
+    rep_ok t ->
+    In (k, v) (elements t) ->
+    bound k t = true /\ get k t = v.
+Proof.
+  intros k v t. simpl. intros Hin.
+  pose proof SearchTree.elements_correct as Hcorrect.
+  unfold elements_correct_spec in Hcorrect.
+  apply Hcorrect; assumption.
+Qed.
+
+End TreeETableEncapsulated.
+
+Module NicelyEncapsulatedExample.
+
+Module StringTreeETableEncapsulated := TreeETableEncapsulated StringVal.
+Import StringTreeETableEncapsulated.
+Open Scope string_scope.
+
+Example ex1 : get 0 empty = "".
+Proof.
+    Fail unfold get. 
+    Fail reflexivity.
+  
+    apply get_empty_default.
+Qed.
+
+End NicelyEncapsulatedExample.
+
+Definition map_update {V : Type} (k : key) (v : V) (m : partial_map V) : partial_map V :=
+  update m k v.
+Definition map_find {V : Type} := @find V.
+Definition empty_map {V : Type} := @Maps.empty V.
+
+Module Type ETableAbs.
+
+  Parameter table : Type.
+  Definition key := nat.
+  Parameter V : Type.
+  Parameter default : V.
+  Parameter empty : table.
+  Parameter get : key -> table -> V.
+  Parameter set : key -> V -> table -> table.
+  Parameter bound : key -> table -> bool.
+  Parameter elements : table -> list (key * V).
+  Parameter Abs : table -> partial_map V.
+  Parameter rep_ok : table -> Prop.
+
+  Axiom empty_ok :
+      rep_ok empty.
+
+  Axiom set_ok : forall (k : key) (v : V) (t : table),
+      rep_ok t -> rep_ok (set k v t).
+
+  Axiom empty_relate :
+      Abs empty = empty_map.
+
+  Axiom bound_relate : forall (t : table) (k : key),
+      rep_ok t ->
+      map_bound k (Abs t) = bound k t.
+
+  Axiom lookup_relate : forall (t : table) (k : key),
+      rep_ok t ->
+      map_find default k (Abs t) = get k t.
+
+  Axiom insert_relate : forall (t : table) (k : key) (v : V),
+      rep_ok t ->
+      map_update k v (Abs t) = Abs (set k v t).
+
+  Axiom elements_relate : forall (t : table),
+      rep_ok t ->
+      Abs t = map_of_list (elements t).
+
+End ETableAbs.
+
+Module ListETableAbs (VT : ValType) <: ETableAbs.
+
+Definition V := VT.V.
+Definition default := VT.default.
+Definition key := nat.
+Definition table := list (key * V).
+Definition empty : table := [].
+
+Fixpoint get (k : key) (t : table) : V :=
+  match t with
+  | (k', v') :: t' => if k =? k' then v' else (get k t')
+  | [] => default
+  end.
+
+Definition set (k : key) (v : V) (t : table) : table := (k,v)::t.
+
+Fixpoint bound (k : key) (t : table) : bool := 
+  match t with
+  | [] => false
+  | (k', v') :: t' => if k =? k' then true
+                      else bound k t'
+  end.
+
+Definition elements (t : table) : list (key * V) := t.
+
+Definition Abs (t : table) : partial_map V := SearchTree.map_of_list t.
+ 
+Definition rep_ok (t : table) : Prop := 
+   forall (P : (key * V) -> Prop), (forall (x : (key * V)), P x) -> Forall P t.
+  
+Theorem empty_ok : rep_ok empty.
+Proof.
+  unfold rep_ok. intros. apply Forall_nil. 
+Qed.
+
+Theorem set_ok : forall (k : key) (v : V) (t : table),
+      rep_ok t -> rep_ok (set k v t).
+Proof.
+  intros.  
+  unfold rep_ok, set.  
+  intros. apply Forall_cons_iff. 
+  unfold rep_ok in H. 
+  split.  
+  - apply H0.
+  - apply H in H0. apply H0. 
+Qed.
+
+Theorem empty_relate :
+   Abs empty = empty_map.
+Proof.
+  unfold Abs. simpl. reflexivity. 
+Qed.
+
+Theorem bound_relate : forall (t : table) (k : key),
+   rep_ok t ->
+   map_bound k (Abs t) = bound k t.
+Proof.
+  intros. induction t. 
+  - simpl.  unfold Abs. simpl.  
+unfold map_bound. rewrite apply_empty. auto.
+  - unfold Abs. simpl. destruct a. unfold map_bound. 
+    destruct (k =? k0) eqn:Heq.
+    + rewrite Nat.eqb_eq in Heq. subst k0. 
+      rewrite update_eq. auto.
+    + rewrite Nat.eqb_sym in Heq.
+      rewrite Nat.eqb_neq in Heq. eapply update_neq  in Heq.
+      rewrite Heq.  apply IHt. unfold rep_ok in H. unfold rep_ok.
+      intros. apply H in H0. apply Forall_cons_iff in H0. 
+      destruct H0. apply H1. 
+Qed.
+
+Theorem lookup_relate : forall (t : table) (k : key),
+   rep_ok t ->
+   map_find default k (Abs t) = get k t.
+Proof.
+  intros. induction t. 
+  - unfold Abs. unfold map_find. unfold find. 
+    simpl. auto. 
+  - unfold Abs. unfold map_find. unfold find. simpl. destruct a. 
+     destruct (k =? k0) eqn:Heq.
+    + rewrite Nat.eqb_eq in Heq. subst k0. 
+      rewrite update_eq. auto.
+    + rewrite Nat.eqb_sym in Heq.
+      rewrite Nat.eqb_neq in Heq. eapply update_neq  in Heq.
+      rewrite Heq.  apply IHt. unfold rep_ok in H. unfold rep_ok.
+      intros. apply H in H0. apply Forall_cons_iff in H0. 
+      destruct H0. apply H1. 
+Qed.
+
+Theorem insert_relate : forall (t : table) (k : key) (v : V),
+   rep_ok t ->
+   map_update k v (Abs t) = Abs (set k v t).
+Proof.
+  intros. induction t. 
+  - unfold Abs. unfold map_update. simpl. auto.
+  - unfold Abs. unfold map_update. simpl. auto.
+Qed.
+
+Theorem elements_relate : forall (t : table),
+      rep_ok t ->
+      Abs t = map_of_list (elements t).
+Proof.
+  intros. induction t. 
+  - unfold Abs. simpl. auto. 
+ - unfold Abs. simpl. auto.
+Qed.
+
+End ListETableAbs.
+
+(* Instantiate functor for sake of autograding. *)
+Module StringListETableAbs := ListETableAbs StringVal.
+
+Module Type Queue.
+  Parameter V : Type.
+  Parameter queue : Type.
+  Parameter empty: queue.
+  Parameter is_empty : queue -> bool.
+  Parameter enq : queue -> V -> queue.
+  Parameter deq : queue -> queue.
+  Parameter peek : V -> queue -> V.
+  Axiom is_empty_empty : is_empty empty = true.
+  Axiom is_empty_nonempty : forall q v, is_empty (enq q v) = false.
+  Axiom peek_empty : forall d, peek d empty = d.
+  Axiom peek_nonempty : forall d q v, peek d (enq q v) = peek v q.
+  Axiom deq_empty : deq empty = empty.
+  Axiom deq_nonempty : forall q v, deq (enq q v) = if is_empty q then q else enq (deq q) v.
+End Queue.
+
+Module ListQueue <: Queue.
+  Definition V := nat. (* for simplicity *)
+  Definition queue := list V.
+  Definition empty : queue := [].
+  Definition is_empty (q : queue) : bool := if ((length q) =? 0) then true else false.
+  Definition enq (q : queue) (v : V) : queue := q ++ [v].  
+  
+  Definition deq (q : queue) : queue := 
+     match q with 
+      | [] => empty
+      | h::q' => q'
+     end.
+  
+  Definition peek (default : V) (q : queue) : V := 
+    match q with 
+      | [] => default
+      | h::q' => h
+     end.
+  
+Theorem is_empty_empty : is_empty empty = true.
+Proof.
+  unfold is_empty. simpl. auto. 
+Qed.
+
+Theorem is_empty_nonempty : forall q v,
+      is_empty (enq q v) = false.
+Proof.
+  intros. unfold is_empty. unfold enq. rewrite last_length. 
+  specialize Nat.neq_succ_0 with (Datatypes.length q).
+  intros. apply Nat.eqb_neq in H. rewrite H. auto. 
+Qed.
+
+Theorem peek_empty : forall d,
+    peek d empty = d.
+Proof.
+  intros. simpl. auto.
+Qed. 
+
+Theorem peek_nonempty : forall d q v,
+   peek d (enq q v) = peek v q.
+Proof.
+  intros. induction q. 
+ - simpl. auto. 
+ - simpl. auto.
+Qed. 
+
+Theorem deq_empty :
+    deq empty = empty.
+Proof.
+  auto. 
+Qed.     
+
+Theorem deq_nonempty : forall q v,
+    deq (enq q v) = if is_empty q then q else enq (deq q) v.
+Proof.
+  intros. induction q. 
+  - simpl. auto. 
+  - simpl. auto.
+Qed.
+
+
+End ListQueue.
+
+Module Type QueueAbs.
+  Parameter V : Type.
+  Parameter queue : Type.
+  Parameter empty : queue.
+  Parameter is_empty : queue -> bool.
+  Parameter enq : queue -> V -> queue.
+  Parameter deq : queue -> queue.
+  Parameter peek : V -> queue -> V.
+  Parameter Abs : queue -> list V.
+  Axiom empty_relate : Abs empty = [].
+  Axiom enq_relate : forall q v, Abs (enq q v) = (Abs q) ++ [v].
+  Axiom peek_relate : forall d q, peek d q = hd d (Abs q).
+  Axiom deq_relate : forall q, Abs (deq q) = tl (Abs q).
+End QueueAbs.
+
+Module TwoListQueueAbs <: QueueAbs.
+
+  Definition V := nat. (* for simplicity *)
+
+  Definition queue : Type := list V * list V.
+  (* (f, b) represents a queue with a front list f and a back list
+     b, where the back list is stored in reverse order. *)
+
+  Definition Abs '((f, b) : queue) : list V :=
+    f ++ (rev b).
+
+  Definition empty : queue :=
+    ([], []).
+
+  Definition is_empty (q: queue) :=
+    match q with
+    | ([], []) => true
+    | _ => false
+    end.
+
+  Definition enq '((f, b) : queue) (v : V) :=
+    (f, v :: b).
+
+  Definition deq (q : queue) :=
+    match q with
+    | ([], []) => ([], [])
+    | ([], b) =>
+      match rev b with
+      | [] => ([], [])
+      | _ :: f => (f, [])
+      end
+    | (_ :: f, b) => (f, b)
+    end.
+
+  Definition peek (d : V) (q : queue) :=
+    match q with
+    | ([], []) => d
+    | ([], b) =>
+      match rev b with
+      | [] => d
+      | v :: _ => v
+      end
+    | (v :: _, _) => v
+    end.
+
+Theorem empty_relate : Abs empty = [].
+Proof.
+
+
+
+
+
+
 
 
 
